Make many RSL implementation files work with Dafny 3.0.0

ironfleet/src/Dafny/Distributed/Impl/RSL/CMessageRefinements.i.dfy
@@ -6,353 +6,360 @@ include "CMessage.i.dfy"
 include "AppInterface.i.dfy"
 
 module LiveRSL__CMessageRefinements_i {
+import opened Native__Io_s
+import opened Native__NativeTypes_i
+import opened Concrete_NodeIdentity_i
+import opened LiveRSL__AppInterface_i
+import opened LiveRSL__CMessage_i
+import opened LiveRSL__CTypes_i
 import opened LiveRSL__Message_i
 import opened LiveRSL__Environment_i
 import opened LiveRSL__Broadcast_i
 import opened Common__NodeIdentity_i
-import opened LiveRSL__CMessage_i
-import opened LiveRSL__AppInterface_i
+import opened Common__UdpClient_i
+import opened Environment_s
+import opened Collections__Sets_i
 
 predicate CMessageIsAbstractable(msg:CMessage)
 {
-    match msg
-        case CMessage_Invalid => true
-        case CMessage_Request(seqno, value) => CAppMessageIsAbstractable(value)
-        case CMessage_1a(ballot) => CBallotIsAbstractable(ballot)
-        case CMessage_1b(ballot, log_truncation_point, votes) => CBallotIsAbstractable(ballot) && COperationNumberIsAbstractable(log_truncation_point) && CVotesIsAbstractable(votes)
-        case CMessage_2a(ballot, opn, value) => CBallotIsAbstractable(ballot) && COperationNumberIsAbstractable(opn) && CRequestBatchIsAbstractable(value)
-        case CMessage_2b(ballot, opn, value) => CBallotIsAbstractable(ballot) && COperationNumberIsAbstractable(opn) && CRequestBatchIsAbstractable(value)
-        case CMessage_Heartbeat(bal_heartbeat, suspicious, opn_ckpt) => CBallotIsAbstractable(bal_heartbeat) && COperationNumberIsAbstractable(opn_ckpt)
-        case CMessage_Reply(seqno, reply) => CAppMessageIsAbstractable(reply)
-        case CMessage_AppStateRequest(bal_state_req, opn_state_req) => CBallotIsAbstractable(bal_state_req) && COperationNumberIsAbstractable(opn_state_req)
-        case CMessage_AppStateSupply(bal_state_supply, opn_state_supply, app_state, reply_cache) => CBallotIsAbstractable(bal_state_supply) && COperationNumberIsAbstractable(opn_state_supply) && CAppStateIsAbstractable(app_state) && CReplyCacheIsAbstractable(reply_cache)
-        case CMessage_StartingPhase2(bal_2, logTruncationPoint_2) => CBallotIsAbstractable(bal_2) && COperationNumberIsAbstractable(logTruncationPoint_2)
+  match msg
+    case CMessage_Invalid => true
+    case CMessage_Request(seqno, value) => CAppMessageIsAbstractable(value)
+    case CMessage_1a(ballot) => CBallotIsAbstractable(ballot)
+    case CMessage_1b(ballot, log_truncation_point, votes) => CBallotIsAbstractable(ballot) && COperationNumberIsAbstractable(log_truncation_point) && CVotesIsAbstractable(votes)
+    case CMessage_2a(ballot, opn, value) => CBallotIsAbstractable(ballot) && COperationNumberIsAbstractable(opn) && CRequestBatchIsAbstractable(value)
+    case CMessage_2b(ballot, opn, value) => CBallotIsAbstractable(ballot) && COperationNumberIsAbstractable(opn) && CRequestBatchIsAbstractable(value)
+    case CMessage_Heartbeat(bal_heartbeat, suspicious, opn_ckpt) => CBallotIsAbstractable(bal_heartbeat) && COperationNumberIsAbstractable(opn_ckpt)
+    case CMessage_Reply(seqno, reply) => CAppMessageIsAbstractable(reply)
+    case CMessage_AppStateRequest(bal_state_req, opn_state_req) => CBallotIsAbstractable(bal_state_req) && COperationNumberIsAbstractable(opn_state_req)
+    case CMessage_AppStateSupply(bal_state_supply, opn_state_supply, app_state, reply_cache) => CBallotIsAbstractable(bal_state_supply) && COperationNumberIsAbstractable(opn_state_supply) && CAppStateIsAbstractable(app_state) && CReplyCacheIsAbstractable(reply_cache)
+    case CMessage_StartingPhase2(bal_2, logTruncationPoint_2) => CBallotIsAbstractable(bal_2) && COperationNumberIsAbstractable(logTruncationPoint_2)
 
 }
 
 function AbstractifyCMessageToRslMessage(msg:CMessage) : RslMessage
-    requires CMessageIsAbstractable(msg);
+  requires CMessageIsAbstractable(msg)
 {
-    match msg
-        case CMessage_Invalid => RslMessage_Invalid()
-        case CMessage_Request(seqno, value) => RslMessage_Request(int(seqno), AbstractifyCAppMessageToAppMessage(value))
-        case CMessage_1a(ballot) => RslMessage_1a(AbstractifyCBallotToBallot(ballot))
-        case CMessage_1b(ballot, log_truncation_point, votes) => RslMessage_1b(AbstractifyCBallotToBallot(ballot), AbstractifyCOperationNumberToOperationNumber(log_truncation_point), AbstractifyCVotesToVotes(votes))
-        case CMessage_2a(ballot, opn, value) => RslMessage_2a(AbstractifyCBallotToBallot(ballot), AbstractifyCOperationNumberToOperationNumber(opn), AbstractifyCRequestBatchToRequestBatch(value))
-        case CMessage_2b(ballot, opn, value) => RslMessage_2b(AbstractifyCBallotToBallot(ballot), AbstractifyCOperationNumberToOperationNumber(opn), AbstractifyCRequestBatchToRequestBatch(value))
-        case CMessage_Heartbeat(bal_heartbeat, suspicious, opn_ckpt) => RslMessage_Heartbeat(AbstractifyCBallotToBallot(bal_heartbeat), suspicious, AbstractifyCOperationNumberToOperationNumber(opn_ckpt))
-        case CMessage_Reply(seqno, reply) => RslMessage_Reply(int(seqno), AbstractifyCAppMessageToAppMessage(reply))
-        case CMessage_AppStateRequest(bal_state_req, opn_state_req) => RslMessage_AppStateRequest(AbstractifyCBallotToBallot(bal_state_req), AbstractifyCOperationNumberToOperationNumber(opn_state_req))
-        case CMessage_AppStateSupply(bal_state_supply, opn_state_supply, app_state, reply_cache) => RslMessage_AppStateSupply(AbstractifyCBallotToBallot(bal_state_supply), AbstractifyCOperationNumberToOperationNumber(opn_state_supply), AbstractifyCAppStateToAppState(app_state), AbstractifyCReplyCacheToReplyCache(reply_cache))
-        case CMessage_StartingPhase2(bal_2, logTruncationPoint_2) => RslMessage_StartingPhase2(AbstractifyCBallotToBallot(bal_2), AbstractifyCOperationNumberToOperationNumber(logTruncationPoint_2))
+  match msg
+    case CMessage_Invalid => RslMessage_Invalid()
+    case CMessage_Request(seqno, value) => RslMessage_Request(seqno as int, AbstractifyCAppMessageToAppMessage(value))
+    case CMessage_1a(ballot) => RslMessage_1a(AbstractifyCBallotToBallot(ballot))
+    case CMessage_1b(ballot, log_truncation_point, votes) => RslMessage_1b(AbstractifyCBallotToBallot(ballot), AbstractifyCOperationNumberToOperationNumber(log_truncation_point), AbstractifyCVotesToVotes(votes))
+    case CMessage_2a(ballot, opn, value) => RslMessage_2a(AbstractifyCBallotToBallot(ballot), AbstractifyCOperationNumberToOperationNumber(opn), AbstractifyCRequestBatchToRequestBatch(value))
+    case CMessage_2b(ballot, opn, value) => RslMessage_2b(AbstractifyCBallotToBallot(ballot), AbstractifyCOperationNumberToOperationNumber(opn), AbstractifyCRequestBatchToRequestBatch(value))
+    case CMessage_Heartbeat(bal_heartbeat, suspicious, opn_ckpt) => RslMessage_Heartbeat(AbstractifyCBallotToBallot(bal_heartbeat), suspicious, AbstractifyCOperationNumberToOperationNumber(opn_ckpt))
+    case CMessage_Reply(seqno, reply) => RslMessage_Reply(seqno as int, AbstractifyCAppMessageToAppMessage(reply))
+    case CMessage_AppStateRequest(bal_state_req, opn_state_req) => RslMessage_AppStateRequest(AbstractifyCBallotToBallot(bal_state_req), AbstractifyCOperationNumberToOperationNumber(opn_state_req))
+    case CMessage_AppStateSupply(bal_state_supply, opn_state_supply, app_state, reply_cache) => RslMessage_AppStateSupply(AbstractifyCBallotToBallot(bal_state_supply), AbstractifyCOperationNumberToOperationNumber(opn_state_supply), AbstractifyCAppStateToAppState(app_state), AbstractifyCReplyCacheToReplyCache(reply_cache))
+    case CMessage_StartingPhase2(bal_2, logTruncationPoint_2) => RslMessage_StartingPhase2(AbstractifyCBallotToBallot(bal_2), AbstractifyCOperationNumberToOperationNumber(logTruncationPoint_2))
 }
 
 function AbstractifyCMessageToRslPacket(sentTo:EndPoint, sentFrom:EndPoint, msg:CMessage) : RslPacket
-    requires CMessageIsAbstractable(msg);
-    requires EndPointIsValidIPV4(sentTo);
-    requires EndPointIsValidIPV4(sentFrom);
+  requires CMessageIsAbstractable(msg)
+  requires EndPointIsValidIPV4(sentTo)
+  requires EndPointIsValidIPV4(sentFrom)
 {
-    LPacket(AbstractifyEndPointToNodeIdentity(sentTo), AbstractifyEndPointToNodeIdentity(sentFrom), AbstractifyCMessageToRslMessage(msg))
+  LPacket(AbstractifyEndPointToNodeIdentity(sentTo), AbstractifyEndPointToNodeIdentity(sentFrom), AbstractifyCMessageToRslMessage(msg))
 }
 
 predicate CPacketIsAbstractable(cp:CPacket)
 {
-       CMessageIsAbstractable(cp.msg)
-    && EndPointIsValidIPV4(cp.src)
-    && EndPointIsValidIPV4(cp.dst)
+  && CMessageIsAbstractable(cp.msg)
+  && EndPointIsValidIPV4(cp.src)
+  && EndPointIsValidIPV4(cp.dst)
 }
 
 predicate CPacketsIsAbstractable(cps:set<CPacket>)
 {
-    forall cp :: cp in cps ==> CPacketIsAbstractable(cp)
+  forall cp :: cp in cps ==> CPacketIsAbstractable(cp)
 }
 
 function AbstractifyCPacketToRslPacket(cp: CPacket): RslPacket
-    ensures CPacketIsAbstractable(cp) ==> AbstractifyCPacketToRslPacket(cp) == LPacket(AbstractifyEndPointToNodeIdentity(cp.dst), AbstractifyEndPointToNodeIdentity(cp.src), AbstractifyCMessageToRslMessage(cp.msg));
+  ensures CPacketIsAbstractable(cp) ==> AbstractifyCPacketToRslPacket(cp) == LPacket(AbstractifyEndPointToNodeIdentity(cp.dst), AbstractifyEndPointToNodeIdentity(cp.src), AbstractifyCMessageToRslMessage(cp.msg))
 {
-    if (CPacketIsAbstractable(cp)) then
+  if (CPacketIsAbstractable(cp)) then
     LPacket(AbstractifyEndPointToNodeIdentity(cp.dst), AbstractifyEndPointToNodeIdentity(cp.src), AbstractifyCMessageToRslMessage(cp.msg))
-    else var x:RslPacket :| (true); x
+  else
+    var x:RslPacket :| (true); x
 }
 
 function AbstractifySetOfCPacketsToSetOfRslPackets_transparent(cps:set<CPacket>) : set<RslPacket>
-    requires CPacketsIsAbstractable(cps);
+  requires CPacketsIsAbstractable(cps)
 {
-    set cp | cp in cps :: AbstractifyCPacketToRslPacket(cp)
+  set cp | cp in cps :: AbstractifyCPacketToRslPacket(cp)
 }
 
 function {:opaque} AbstractifySetOfCPacketsToSetOfRslPackets(cps:set<CPacket>) : set<RslPacket>
-    requires CPacketsIsAbstractable(cps);
-    //ensures forall p :: p in cps ==> AbstractifyCPacketToRslPacket(p) in AbstractifySetOfCPacketsToSetOfRslPackets(cps);   // Still too trigger happy
+  requires CPacketsIsAbstractable(cps)
+  //ensures forall p :: p in cps ==> AbstractifyCPacketToRslPacket(p) in AbstractifySetOfCPacketsToSetOfRslPackets(cps)   // Still too trigger happy
 {
- //   set udpp | udpp in udpps ::
- //       var udp := AbstractifyCPacketToShtPacket(udpp); udp
-    AbstractifySetOfCPacketsToSetOfRslPackets_transparent(cps)
+//  set udpp | udpp in udpps ::
+//    var udp := AbstractifyCPacketToShtPacket(udpp); udp
+  AbstractifySetOfCPacketsToSetOfRslPackets_transparent(cps)
 }
 
 predicate CPacketSeqIsAbstractable(cps:seq<CPacket>)
 {
-    forall i :: 0 <= i < |cps| ==> CPacketIsAbstractable(cps[i])
+  forall i :: 0 <= i < |cps| ==> CPacketIsAbstractable(cps[i])
 }
 
 function {:opaque} AbstractifySeqOfCPacketsToSeqOfRslPackets(cps:seq<CPacket>) : seq<RslPacket>
-    requires CPacketSeqIsAbstractable(cps);
-    ensures |cps| == |AbstractifySeqOfCPacketsToSeqOfRslPackets(cps)|;
-    ensures forall i :: 0 <= i < |cps| ==> AbstractifySeqOfCPacketsToSeqOfRslPackets(cps)[i] == AbstractifyCPacketToRslPacket(cps[i]);
+  requires CPacketSeqIsAbstractable(cps)
+  ensures |cps| == |AbstractifySeqOfCPacketsToSeqOfRslPackets(cps)|
+  ensures forall i :: 0 <= i < |cps| ==> AbstractifySeqOfCPacketsToSeqOfRslPackets(cps)[i] == AbstractifyCPacketToRslPacket(cps[i])
 {
-    if |cps| == 0 then []
-    else [AbstractifyCPacketToRslPacket(cps[0])] + AbstractifySeqOfCPacketsToSeqOfRslPackets(cps[1..])
+  if |cps| == 0 then []
+  else [AbstractifyCPacketToRslPacket(cps[0])] + AbstractifySeqOfCPacketsToSeqOfRslPackets(cps[1..])
 }
 
 predicate CPacketSeqHasCorrectSrc(sent_packets:seq<CPacket>, me:EndPoint)
 {
-    forall p :: p in sent_packets ==> p.src == me
+  forall p :: p in sent_packets ==> p.src == me
 }
 
 
 predicate CMessageIsInjectiveType(m:CMessage)
 {
-       CMessageIsAbstractable(m)
-    && (m.CMessage_1b? || m.CMessage_2b?)
+  && CMessageIsAbstractable(m)
+  && (m.CMessage_1b? || m.CMessage_2b?)
 }
 
 lemma lemma_AbstractifyCMessageToRslMessage_isInjective(m1:CMessage, m2:CMessage)
-    requires CMessageIsInjectiveType(m1) && CMessageIsInjectiveType(m2)
-    requires AbstractifyCMessageToRslMessage(m1) == AbstractifyCMessageToRslMessage(m2);
-    ensures m1 == m2;
+  requires CMessageIsInjectiveType(m1) && CMessageIsInjectiveType(m2)
+  requires AbstractifyCMessageToRslMessage(m1) == AbstractifyCMessageToRslMessage(m2)
+  ensures m1 == m2
 {
-    lemma_AbstractifyCRequestBatchToRequestBatch_isInjective();
+  lemma_AbstractifyCRequestBatchToRequestBatch_isInjective();
 
-    if (m1.CMessage_1b?) {
-        lemma_BallotInjective(m1.bal_1b, m2.bal_1b);
-        lemma_VotesInjective(m1.votes, m2.votes);
-        assert m1 == m2;
-    } else if (m1.CMessage_2b?) {
-        lemma_BallotInjective(m1.bal_2b, m2.bal_2b);
-        assert AbstractifyCRequestBatchToRequestBatch(m1.val_2b) == AbstractifyCRequestBatchToRequestBatch(m2.val_2b);
-        assert m1 == m2;
-    }
+  if (m1.CMessage_1b?) {
+    lemma_BallotInjective(m1.bal_1b, m2.bal_1b);
+    lemma_VotesInjective(m1.votes, m2.votes);
+    assert m1 == m2;
+  } else if (m1.CMessage_2b?) {
+    lemma_BallotInjective(m1.bal_2b, m2.bal_2b);
+    assert AbstractifyCRequestBatchToRequestBatch(m1.val_2b) == AbstractifyCRequestBatchToRequestBatch(m2.val_2b);
+    assert m1 == m2;
+  }
 }
 
 predicate CPacketIsInjectiveType(p:CPacket)
 {
-    CPacketIsAbstractable(p) && CMessageIsInjectiveType(p.msg)
+  CPacketIsAbstractable(p) && CMessageIsInjectiveType(p.msg)
 }
 
 lemma lemma_AbstractifyCPacketToRslPacket_isInjective()
-    ensures forall p1, p2 ::
-           CPacketIsInjectiveType(p1) && CPacketIsInjectiveType(p2)
-        && AbstractifyCPacketToRslPacket(p1) == AbstractifyCPacketToRslPacket(p2)
-        ==> p1 == p2
+  ensures forall p1, p2 ::
+            && CPacketIsInjectiveType(p1)
+            && CPacketIsInjectiveType(p2)
+            && AbstractifyCPacketToRslPacket(p1) == AbstractifyCPacketToRslPacket(p2)
+            ==> p1 == p2
 {
-    forall p1, p2 | CPacketIsInjectiveType(p1) && CPacketIsInjectiveType(p2)
-        && AbstractifyCPacketToRslPacket(p1) == AbstractifyCPacketToRslPacket(p2)
-        ensures p1 == p2;
-    {
-        lemma_AbstractifyEndPointToNodeIdentity_injective_forall();
-        lemma_AbstractifyCMessageToRslMessage_isInjective(p1.msg, p2.msg);
-    }
+  forall p1, p2 |
+    && CPacketIsInjectiveType(p1)
+    && CPacketIsInjectiveType(p2)
+    && AbstractifyCPacketToRslPacket(p1) == AbstractifyCPacketToRslPacket(p2)
+    ensures p1 == p2
+  {
+    lemma_AbstractifyEndPointToNodeIdentity_injective_forall();
+    lemma_AbstractifyCMessageToRslMessage_isInjective(p1.msg, p2.msg);
+  }
 }
 
 predicate SetOfInjectiveTypeCPackets(s:set<CPacket>)
 {
-    forall p :: p in s ==> CPacketIsInjectiveType(p)
+  forall p :: p in s ==> CPacketIsInjectiveType(p)
 }
 
 predicate SetOfInjectiveTypeCPacketsIsInjective(s:set<CPacket>)
 {
-       SetOfInjectiveTypeCPackets(s)
-    && forall p1, p2 :: p1 in s && p2 in s &&  AbstractifyCPacketToRslPacket(p1) == AbstractifyCPacketToRslPacket(p2)
-        ==> p1 == p2
+  && SetOfInjectiveTypeCPackets(s)
+  && (forall p1, p2 :: p1 in s && p2 in s && AbstractifyCPacketToRslPacket(p1) == AbstractifyCPacketToRslPacket(p2)
+        ==> p1 == p2)
 }
 
 lemma lemma_SetOfInjectiveTypeCPacketsIsInjective(s:set<CPacket>)
-    requires SetOfInjectiveTypeCPackets(s);
-    ensures SetOfInjectiveTypeCPacketsIsInjective(s);
+  requires SetOfInjectiveTypeCPackets(s)
+  ensures SetOfInjectiveTypeCPacketsIsInjective(s)
 {
-    lemma_AbstractifyCPacketToRslPacket_isInjective();
+  lemma_AbstractifyCPacketToRslPacket_isInjective();
 }
 
 lemma lemma_AbstractifySetOfCPacketsToSetOfRslPackets_isInjective(cps1:set<CPacket>, cps2:set<CPacket>)
-    requires CPacketsIsAbstractable(cps1);
-    requires CPacketsIsAbstractable(cps2);
-    requires SetOfInjectiveTypeCPackets(cps1);
-    requires SetOfInjectiveTypeCPackets(cps2);
-    requires AbstractifySetOfCPacketsToSetOfRslPackets(cps1) == AbstractifySetOfCPacketsToSetOfRslPackets(cps2);
-    ensures  cps1 == cps2;
+  requires CPacketsIsAbstractable(cps1)
+  requires CPacketsIsAbstractable(cps2)
+  requires SetOfInjectiveTypeCPackets(cps1)
+  requires SetOfInjectiveTypeCPackets(cps2)
+  requires AbstractifySetOfCPacketsToSetOfRslPackets(cps1) == AbstractifySetOfCPacketsToSetOfRslPackets(cps2)
+  ensures  cps1 == cps2
 {
-    reveal_AbstractifySetOfCPacketsToSetOfRslPackets();
-    lemma_AbstractifyCPacketToRslPacket_isInjective();
-    forall cp1 | cp1 in cps1
-        ensures cp1 in cps2;
-    {
-        var p := AbstractifyCPacketToRslPacket(cp1);
-        assert p in AbstractifySetOfCPacketsToSetOfRslPackets(cps2);
-    }
-    forall cp2 | cp2 in cps2
-        ensures cp2 in cps1;
-    {
-        var p := AbstractifyCPacketToRslPacket(cp2);
-        assert p in AbstractifySetOfCPacketsToSetOfRslPackets(cps1);
-    }
+  reveal AbstractifySetOfCPacketsToSetOfRslPackets();
+  lemma_AbstractifyCPacketToRslPacket_isInjective();
+  forall cp1 | cp1 in cps1
+    ensures cp1 in cps2
+  {
+    var p := AbstractifyCPacketToRslPacket(cp1);
+    assert p in AbstractifySetOfCPacketsToSetOfRslPackets(cps2);
+  }
+  forall cp2 | cp2 in cps2
+    ensures cp2 in cps1
+  {
+    var p := AbstractifyCPacketToRslPacket(cp2);
+    assert p in AbstractifySetOfCPacketsToSetOfRslPackets(cps1);
+  }
 }
 
 lemma lemma_AbstractifySetOfCPacketsToSetOfRslPackets_cardinality(cps:set<CPacket>)
-    requires CPacketsIsAbstractable(cps);
-    requires SetOfInjectiveTypeCPackets(cps);
-    ensures  |cps| == |AbstractifySetOfCPacketsToSetOfRslPackets(cps)|;
+  requires CPacketsIsAbstractable(cps)
+  requires SetOfInjectiveTypeCPackets(cps)
+  ensures  |cps| == |AbstractifySetOfCPacketsToSetOfRslPackets(cps)|
 {
-    lemma_SetOfInjectiveTypeCPacketsIsInjective(cps);
-    var rps := AbstractifySetOfCPacketsToSetOfRslPackets(cps);
-    forall y | y in rps 
-        ensures exists x :: x in cps && y == AbstractifyCPacketToRslPacket(x);
-    {
-        reveal_AbstractifySetOfCPacketsToSetOfRslPackets();
-    }
+  lemma_SetOfInjectiveTypeCPacketsIsInjective(cps);
+  var rps := AbstractifySetOfCPacketsToSetOfRslPackets(cps);
+  forall y | y in rps 
+    ensures exists x :: x in cps && y == AbstractifyCPacketToRslPacket(x)
+  {
+    reveal AbstractifySetOfCPacketsToSetOfRslPackets();
+  }
 
-    forall x | x in cps 
-        ensures AbstractifyCPacketToRslPacket(x) in rps;
-    {
-        reveal_AbstractifySetOfCPacketsToSetOfRslPackets();
-    }
-    lemma_MapSetCardinalityOver(cps, rps, AbstractifyCPacketToRslPacket);
+  forall x | x in cps 
+    ensures AbstractifyCPacketToRslPacket(x) in rps
+  {
+    reveal AbstractifySetOfCPacketsToSetOfRslPackets();
+  }
+  lemma_MapSetCardinalityOver(cps, rps, AbstractifyCPacketToRslPacket);
 }
 
 
 lemma lemma_AbstractifySetOfCPacketsToSetOfRslPackets_properties(cps:set<CPacket>)
-    requires CPacketsIsAbstractable(cps);
-    ensures  SetOfInjectiveTypeCPackets(cps) ==> |cps| == |AbstractifySetOfCPacketsToSetOfRslPackets(cps)|;
-    ensures  AbstractifySetOfCPacketsToSetOfRslPackets({}) == {};
+  requires CPacketsIsAbstractable(cps)
+  ensures  SetOfInjectiveTypeCPackets(cps) ==> |cps| == |AbstractifySetOfCPacketsToSetOfRslPackets(cps)|
+  ensures  AbstractifySetOfCPacketsToSetOfRslPackets({}) == {}
 {
-    if SetOfInjectiveTypeCPackets(cps) {
-        lemma_AbstractifySetOfCPacketsToSetOfRslPackets_cardinality(cps);
-    }
+  if SetOfInjectiveTypeCPackets(cps) {
+    lemma_AbstractifySetOfCPacketsToSetOfRslPackets_cardinality(cps);
+  }
 
-    reveal_AbstractifySetOfCPacketsToSetOfRslPackets();
+  reveal AbstractifySetOfCPacketsToSetOfRslPackets();
 }
 
 lemma lemma_AbstractifyCPacketToRslPacket_src(cps:set<CPacket>, src:EndPoint)
-    requires CPacketsIsAbstractable(cps);
-    requires EndPointIsValidIPV4(src);
-    requires forall p :: p in AbstractifySetOfCPacketsToSetOfRslPackets(cps) ==> p.src == AbstractifyEndPointToNodeIdentity(src);
-    ensures  forall cp :: cp in cps ==> cp.src == src;
+  requires CPacketsIsAbstractable(cps)
+  requires EndPointIsValidIPV4(src)
+  requires forall p :: p in AbstractifySetOfCPacketsToSetOfRslPackets(cps) ==> p.src == AbstractifyEndPointToNodeIdentity(src)
+  ensures  forall cp :: cp in cps ==> cp.src == src
 {
-    reveal_AbstractifySetOfCPacketsToSetOfRslPackets();
-    lemma_Uint64EndPointRelationships();
-    lemma_AbstractifyEndPointToNodeIdentity_injective_forall();
-    forall cp | cp in cps
-        ensures cp.src == src;
-    {
-        assert AbstractifyCPacketToRslPacket(cp).src == AbstractifyEndPointToNodeIdentity(src);
-        assert cp.src == src;
-    }
+  reveal AbstractifySetOfCPacketsToSetOfRslPackets();
+  lemma_Uint64EndPointRelationships();
+  lemma_AbstractifyEndPointToNodeIdentity_injective_forall();
+  forall cp | cp in cps
+    ensures cp.src == src
+  {
+    assert AbstractifyCPacketToRslPacket(cp).src == AbstractifyEndPointToNodeIdentity(src);
+    assert cp.src == src;
+  }
 }
 
 lemma lemma_AbstractifySetOfCPacketsToSetOfRslPackets_srcMembershipNeg(cps:set<CPacket>, src:EndPoint)
-    requires CPacketsIsAbstractable(cps);
-    requires EndPointIsValidIPV4(src);
-    requires !(forall p :: p in cps ==> p.src != src);
-    ensures  !(forall p :: p in AbstractifySetOfCPacketsToSetOfRslPackets(cps) ==> p.src != AbstractifyEndPointToNodeIdentity(src));
+  requires CPacketsIsAbstractable(cps)
+  requires EndPointIsValidIPV4(src)
+  requires !(forall p :: p in cps ==> p.src != src)
+  ensures  !(forall p :: p in AbstractifySetOfCPacketsToSetOfRslPackets(cps) ==> p.src != AbstractifyEndPointToNodeIdentity(src))
 {
-    assert exists p :: p in cps && p.src == src;
-    var cp :| cp in cps && cp.src == src;
-    var p := AbstractifyCPacketToRslPacket(cp);
-    reveal_AbstractifySetOfCPacketsToSetOfRslPackets();
-    assert p in AbstractifySetOfCPacketsToSetOfRslPackets(cps);
-    lemma_AbstractifyEndPointToNodeIdentity_injective_forall();
+  assert exists p :: p in cps && p.src == src;
+  var cp :| cp in cps && cp.src == src;
+  var p := AbstractifyCPacketToRslPacket(cp);
+  reveal AbstractifySetOfCPacketsToSetOfRslPackets();
+  assert p in AbstractifySetOfCPacketsToSetOfRslPackets(cps);
+  lemma_AbstractifyEndPointToNodeIdentity_injective_forall();
 }
 
 lemma lemma_AbstractifySetOfCPacketsToSetOfRslPackets_srcMembershipPos(cps:set<CPacket>, src:EndPoint)
-    requires CPacketsIsAbstractable(cps);
-    requires EndPointIsValidIPV4(src);
-    requires forall p :: p in cps ==> p.src != src;
-    ensures  forall p :: p in AbstractifySetOfCPacketsToSetOfRslPackets(cps) ==> p.src != AbstractifyEndPointToNodeIdentity(src);
+  requires CPacketsIsAbstractable(cps)
+  requires EndPointIsValidIPV4(src)
+  requires forall p :: p in cps ==> p.src != src
+  ensures  forall p :: p in AbstractifySetOfCPacketsToSetOfRslPackets(cps) ==> p.src != AbstractifyEndPointToNodeIdentity(src)
 {
-    forall p | p in AbstractifySetOfCPacketsToSetOfRslPackets(cps)
-        ensures p.src != AbstractifyEndPointToNodeIdentity(src);
-    {
-        reveal_AbstractifySetOfCPacketsToSetOfRslPackets();
-        var cp :| cp in cps && AbstractifyCPacketToRslPacket(cp) == p;
-        assert p.src == AbstractifyEndPointToNodeIdentity(cp.src);
-        assert cp.src != src;
-        lemma_AbstractifyEndPointToNodeIdentity_injective_forall();
-    }
+  forall p | p in AbstractifySetOfCPacketsToSetOfRslPackets(cps)
+    ensures p.src != AbstractifyEndPointToNodeIdentity(src)
+  {
+    reveal AbstractifySetOfCPacketsToSetOfRslPackets();
+    var cp :| cp in cps && AbstractifyCPacketToRslPacket(cp) == p;
+    assert p.src == AbstractifyEndPointToNodeIdentity(cp.src);
+    assert cp.src != src;
+    lemma_AbstractifyEndPointToNodeIdentity_injective_forall();
+  }
 }
 
 lemma lemma_AbstractifySetOfCPacketsToSetOfRslPackets_srcMembership(cps:set<CPacket>, src:EndPoint)
-    requires CPacketsIsAbstractable(cps);
-    requires EndPointIsValidIPV4(src);
-    ensures  (forall p :: p in cps ==> p.src != src) <==> (forall p :: p in AbstractifySetOfCPacketsToSetOfRslPackets(cps) ==> p.src != AbstractifyEndPointToNodeIdentity(src));
+  requires CPacketsIsAbstractable(cps)
+  requires EndPointIsValidIPV4(src)
+  ensures  (forall p :: p in cps ==> p.src != src) <==> (forall p :: p in AbstractifySetOfCPacketsToSetOfRslPackets(cps) ==> p.src != AbstractifyEndPointToNodeIdentity(src))
 {
-    var b := (forall p :: p in cps ==> p.src != src);
+  var b := (forall p :: p in cps ==> p.src != src);
 
-    if b {
-        lemma_AbstractifySetOfCPacketsToSetOfRslPackets_srcMembershipPos(cps, src);
-    } else {
-        lemma_AbstractifySetOfCPacketsToSetOfRslPackets_srcMembershipNeg(cps, src);
-    }
+  if b {
+    lemma_AbstractifySetOfCPacketsToSetOfRslPackets_srcMembershipPos(cps, src);
+  } else {
+    lemma_AbstractifySetOfCPacketsToSetOfRslPackets_srcMembershipNeg(cps, src);
+  }
 }
 
 
 function {:opaque} BuildLBroadcast(src:NodeIdentity, dsts:seq<NodeIdentity>, m:RslMessage):seq<RslPacket>
-    ensures |BuildLBroadcast(src, dsts, m)| == |dsts|;
-    ensures forall i :: 0 <= i < |dsts| ==> BuildLBroadcast(src, dsts, m)[i] == LPacket(dsts[i], src, m);
+  ensures |BuildLBroadcast(src, dsts, m)| == |dsts|
+  ensures forall i :: 0 <= i < |dsts| ==> BuildLBroadcast(src, dsts, m)[i] == LPacket(dsts[i], src, m)
 {
-    if |dsts| == 0 then []
-    else [LPacket(dsts[0], src, m)] + BuildLBroadcast(src, dsts[1..], m)
+  if |dsts| == 0 then []
+  else [LPacket(dsts[0], src, m)] + BuildLBroadcast(src, dsts[1..], m)
 }
 
 predicate CBroadcastIsAbstractable(broadcast:CBroadcast) 
 {
-    broadcast.CBroadcastNop? ||
-    (   broadcast.CBroadcast? 
+  || broadcast.CBroadcastNop?
+  || (&& broadcast.CBroadcast? 
      && EndPointIsValidIPV4(broadcast.src)
      && (forall i :: 0 <= i < |broadcast.dsts| ==> EndPointIsValidIPV4(broadcast.dsts[i]))
      && CMessageIsAbstractable(broadcast.msg))
 }
 
 function AbstractifyCBroadcastToRlsPacketSeq(broadcast:CBroadcast) : seq<RslPacket>
-    requires CBroadcastIsAbstractable(broadcast);
+  requires CBroadcastIsAbstractable(broadcast)
 {
-    match broadcast {
-        case CBroadcast(_,_,_) => BuildLBroadcast(AbstractifyEndPointToNodeIdentity(broadcast.src), 
-                                                  AbstractifyEndPointsToNodeIdentities(broadcast.dsts), 
-                                                  AbstractifyCMessageToRslMessage(broadcast.msg))
-        case CBroadcastNop => []
-    }
+  match broadcast
+    case CBroadcast(_,_,_) => BuildLBroadcast(AbstractifyEndPointToNodeIdentity(broadcast.src), 
+                                              AbstractifyEndPointsToNodeIdentities(broadcast.dsts), 
+                                              AbstractifyCMessageToRslMessage(broadcast.msg))
+    case CBroadcastNop => []
 }
 
 predicate OutboundPacketsIsAbstractable(out:OutboundPackets)
 {
-    match out {
-        case Broadcast(broadcast) => CBroadcastIsAbstractable(broadcast)
-        case OutboundPacket(Some(p)) => CPacketIsAbstractable(p)
-        case OutboundPacket(None()) => true
-        case PacketSequence(s) => CPacketSeqIsAbstractable(s)
-    }
+  match out
+    case Broadcast(broadcast) => CBroadcastIsAbstractable(broadcast)
+    case OutboundPacket(Some(p)) => CPacketIsAbstractable(p)
+    case OutboundPacket(None()) => true
+    case PacketSequence(s) => CPacketSeqIsAbstractable(s)
 } 
 
 function AbstractifyOutboundCPacketsToSeqOfRslPackets(out:OutboundPackets) : seq<RslPacket>
     requires OutboundPacketsIsAbstractable(out);
 {
-    match out {
-        case Broadcast(broadcast) => AbstractifyCBroadcastToRlsPacketSeq(broadcast)
-        case OutboundPacket(Some(p)) => [AbstractifyCPacketToRslPacket(p)]
-        case OutboundPacket(None()) => [] 
-        case PacketSequence(s) => AbstractifySeqOfCPacketsToSeqOfRslPackets(s)
-    }
+  match out
+    case Broadcast(broadcast) => AbstractifyCBroadcastToRlsPacketSeq(broadcast)
+    case OutboundPacket(Some(p)) => [AbstractifyCPacketToRslPacket(p)]
+    case OutboundPacket(None()) => [] 
+    case PacketSequence(s) => AbstractifySeqOfCPacketsToSeqOfRslPackets(s)
 } 
 
 predicate OutboundPacketsHasCorrectSrc(out:OutboundPackets, me:EndPoint)
 {
-    match out {
-        case Broadcast(CBroadcast(src, _, _)) => src == me
-        case Broadcast(CBroadcastNop()) => true
-        case OutboundPacket(p) => p.Some? ==> p.v.src == me
-        case PacketSequence(s) => (forall p :: p in s ==> p.src == me)
-//        case OutboundPacket(Some(p)) => p.src == me
-//        case OutboundPacket(None()) => true
-    }
+  match out
+    case Broadcast(CBroadcast(src, _, _)) => src == me
+    case Broadcast(CBroadcastNop()) => true
+    case OutboundPacket(p) => p.Some? ==> p.v.src == me
+    case PacketSequence(s) => (forall p :: p in s ==> p.src == me)
+//    case OutboundPacket(Some(p)) => p.src == me
+//    case OutboundPacket(None()) => true
 }
 
 }
