ironfleet/src/Dafny/Distributed/Impl/RSL/ProposerLemmas.i.dfy
@@ -1,133 +1,140 @@
 include "ProposerState.i.dfy"
 
 module LiveRSL__ProposerLemmas_i {
+import opened Native__Io_s
+import opened LiveRSL__CMessage_i
+import opened LiveRSL__CMessageRefinements_i
+import opened LiveRSL__CTypes_i
+import opened LiveRSL__Proposer_i
 import opened LiveRSL__ProposerState_i
+import opened Collections__Sets_i
+import opened Common__SeqIsUnique_i
 
 predicate SetOfMessage1b(S:set<CPacket>)
 {
-    forall p :: p in S ==> p.msg.CMessage_1b?
+  forall p :: p in S ==> p.msg.CMessage_1b?
 }
 
 predicate SetOfMessage1bAboutBallot(S:set<CPacket>, b:CBallot)
 {
-    SetOfMessage1b(S)
-    && (forall p :: p in S ==> p.msg.bal_1b == b)
+  && SetOfMessage1b(S)
+  && (forall p :: p in S ==> p.msg.bal_1b == b)
 }
 
 predicate IsAfterLogTruncationPoint(opn:COperationNumber, received_1b_packets:set<CPacket>)
 {
-    (forall p :: p in received_1b_packets && p.msg.CMessage_1b? ==> p.msg.log_truncation_point.n <= opn.n)
+  forall p :: p in received_1b_packets && p.msg.CMessage_1b? ==> p.msg.log_truncation_point.n <= opn.n
 }
 
 predicate AllAcceptorsHadNoProposal(S:set<CPacket>, opn:COperationNumber)
-    requires SetOfMessage1b(S);
+  requires SetOfMessage1b(S)
 {
-    forall p :: p in S ==> !(opn in p.msg.votes.v)
+  forall p :: p in S ==> !(opn in p.msg.votes.v)
 }
 
 lemma lemma_AbstractifySetOfCPacketsToSetOfRslPackets_propertiesProposer(cps:set<CPacket>)
-    requires CPacketsIsAbstractable(cps);
-    ensures  SetOfInjectiveTypeCPackets(cps) ==> |cps| == |AbstractifySetOfCPacketsToSetOfRslPackets(cps)|;
-    ensures  AbstractifySetOfCPacketsToSetOfRslPackets({}) == {};
-    ensures  SetOfMessage1b(cps) ==> LSetOfMessage1b(AbstractifySetOfCPacketsToSetOfRslPackets(cps));
-    ensures  forall bal :: CBallotIsAbstractable(bal) ==> SetOfMessage1bAboutBallot(cps, bal) ==> LSetOfMessage1bAboutBallot(AbstractifySetOfCPacketsToSetOfRslPackets(cps), AbstractifyCBallotToBallot(bal));
-    ensures  forall opn :: COperationNumberIsAbstractable(opn) ==> IsAfterLogTruncationPoint(opn, cps) ==> LIsAfterLogTruncationPoint(AbstractifyCOperationNumberToOperationNumber(opn), AbstractifySetOfCPacketsToSetOfRslPackets(cps))
-    ensures  forall opn :: COperationNumberIsAbstractable(opn) ==> !IsAfterLogTruncationPoint(opn, cps) ==> !LIsAfterLogTruncationPoint(AbstractifyCOperationNumberToOperationNumber(opn), AbstractifySetOfCPacketsToSetOfRslPackets(cps))
-    ensures  SetOfMessage1b(cps) ==>
+  requires CPacketsIsAbstractable(cps)
+  ensures  SetOfInjectiveTypeCPackets(cps) ==> |cps| == |AbstractifySetOfCPacketsToSetOfRslPackets(cps)|
+  ensures  AbstractifySetOfCPacketsToSetOfRslPackets({}) == {}
+  ensures  SetOfMessage1b(cps) ==> LSetOfMessage1b(AbstractifySetOfCPacketsToSetOfRslPackets(cps))
+  ensures  forall bal :: CBallotIsAbstractable(bal) ==> SetOfMessage1bAboutBallot(cps, bal) ==> LSetOfMessage1bAboutBallot(AbstractifySetOfCPacketsToSetOfRslPackets(cps), AbstractifyCBallotToBallot(bal))
+  ensures  forall opn :: COperationNumberIsAbstractable(opn) ==> IsAfterLogTruncationPoint(opn, cps) ==> LIsAfterLogTruncationPoint(AbstractifyCOperationNumberToOperationNumber(opn), AbstractifySetOfCPacketsToSetOfRslPackets(cps))
+  ensures  forall opn :: COperationNumberIsAbstractable(opn) ==> !IsAfterLogTruncationPoint(opn, cps) ==> !LIsAfterLogTruncationPoint(AbstractifyCOperationNumberToOperationNumber(opn), AbstractifySetOfCPacketsToSetOfRslPackets(cps))
+  ensures  SetOfMessage1b(cps) ==>
              (forall opn :: COperationNumberIsAbstractable(opn) ==> 
-              AllAcceptorsHadNoProposal(cps, opn) ==> LAllAcceptorsHadNoProposal(AbstractifySetOfCPacketsToSetOfRslPackets(cps), AbstractifyCOperationNumberToOperationNumber(opn)));
-    ensures  SetOfMessage1b(cps) ==>
+              AllAcceptorsHadNoProposal(cps, opn) ==> LAllAcceptorsHadNoProposal(AbstractifySetOfCPacketsToSetOfRslPackets(cps), AbstractifyCOperationNumberToOperationNumber(opn)))
+  ensures  SetOfMessage1b(cps) ==>
              (forall opn :: COperationNumberIsAbstractable(opn) ==> 
-              !AllAcceptorsHadNoProposal(cps, opn) ==> !LAllAcceptorsHadNoProposal(AbstractifySetOfCPacketsToSetOfRslPackets(cps), AbstractifyCOperationNumberToOperationNumber(opn)));
+              !AllAcceptorsHadNoProposal(cps, opn) ==> !LAllAcceptorsHadNoProposal(AbstractifySetOfCPacketsToSetOfRslPackets(cps), AbstractifyCOperationNumberToOperationNumber(opn)))
 {
-    lemma_AbstractifySetOfCPacketsToSetOfRslPackets_properties(cps);
-    if SetOfInjectiveTypeCPackets(cps) {
-        lemma_AbstractifySetOfCPacketsToSetOfRslPackets_cardinality(cps);
-    }
+  lemma_AbstractifySetOfCPacketsToSetOfRslPackets_properties(cps);
+  if SetOfInjectiveTypeCPackets(cps) {
+    lemma_AbstractifySetOfCPacketsToSetOfRslPackets_cardinality(cps);
+  }
 
-    reveal_AbstractifySetOfCPacketsToSetOfRslPackets();
+  reveal AbstractifySetOfCPacketsToSetOfRslPackets();
+
+  forall opn | COperationNumberIsAbstractable(opn) 
+    ensures !IsAfterLogTruncationPoint(opn, cps) ==> !LIsAfterLogTruncationPoint(AbstractifyCOperationNumberToOperationNumber(opn), AbstractifySetOfCPacketsToSetOfRslPackets(cps))
+  {
+    if !IsAfterLogTruncationPoint(opn, cps) {
+      //if |cps| > 0 && (exists p :: p in cps && p.msg.CMessage_1b?)
+      var p :| p in cps && p.msg.CMessage_1b? && p.msg.log_truncation_point.n > opn.n;
+      var ref_p := AbstractifyCPacketToRslPacket(p);
+
+      assert ref_p in AbstractifySetOfCPacketsToSetOfRslPackets(cps);
+      assert ref_p.msg.RslMessage_1b?;
+      assert ref_p.msg.log_truncation_point > AbstractifyCOperationNumberToOperationNumber(opn);
+    }
+  }
+
+  if SetOfMessage1b(cps) {
+    var ref_cps := AbstractifySetOfCPacketsToSetOfRslPackets(cps);
+    forall opn | COperationNumberIsAbstractable(opn) 
+      ensures AllAcceptorsHadNoProposal(cps, opn) ==> LAllAcceptorsHadNoProposal(ref_cps, AbstractifyCOperationNumberToOperationNumber(opn))
+    {
+      var ref_opn := AbstractifyCOperationNumberToOperationNumber(opn);
+      if AllAcceptorsHadNoProposal(cps, opn) {
+        forall rp | rp in ref_cps
+          ensures !(ref_opn in rp.msg.votes)
+        {
+          reveal AbstractifyCVotesToVotes();
+          var p :| p in cps && rp == AbstractifyCPacketToRslPacket(p);
+          if ref_opn in rp.msg.votes {
+            assert opn in p.msg.votes.v;
+            assert false;
+          }
+        }
+
+      }
+    }
 
     forall opn | COperationNumberIsAbstractable(opn) 
-        ensures !IsAfterLogTruncationPoint(opn, cps) ==> !LIsAfterLogTruncationPoint(AbstractifyCOperationNumberToOperationNumber(opn), AbstractifySetOfCPacketsToSetOfRslPackets(cps));
+      ensures !AllAcceptorsHadNoProposal(cps, opn) ==> !LAllAcceptorsHadNoProposal(ref_cps, AbstractifyCOperationNumberToOperationNumber(opn))
     {
-        if !IsAfterLogTruncationPoint(opn, cps) {
-            //if |cps| > 0 && (exists p :: p in cps && p.msg.CMessage_1b?)
-            var p :| p in cps && p.msg.CMessage_1b? && p.msg.log_truncation_point.n > opn.n;
-            var ref_p := AbstractifyCPacketToRslPacket(p);
+      var ref_opn := AbstractifyCOperationNumberToOperationNumber(opn);
+      if !AllAcceptorsHadNoProposal(cps, opn) {
+        assert !(forall p :: p in cps ==> !(opn in p.msg.votes.v));
+        var p :| p in cps && opn in p.msg.votes.v;
+        var ref_p := AbstractifyCPacketToRslPacket(p);
 
-            assert ref_p in AbstractifySetOfCPacketsToSetOfRslPackets(cps);
-            assert ref_p.msg.RslMessage_1b?;
-            assert ref_p.msg.log_truncation_point > AbstractifyCOperationNumberToOperationNumber(opn);
-        }
+        reveal AbstractifyCVotesToVotes();
+
+        assert ref_p in ref_cps;
+      }
     }
+  }
 
-    if SetOfMessage1b(cps) {
-        var ref_cps := AbstractifySetOfCPacketsToSetOfRslPackets(cps);
-        forall opn | COperationNumberIsAbstractable(opn) 
-            ensures AllAcceptorsHadNoProposal(cps, opn) ==> LAllAcceptorsHadNoProposal(ref_cps, AbstractifyCOperationNumberToOperationNumber(opn));
-        {
-            var ref_opn := AbstractifyCOperationNumberToOperationNumber(opn);
-            if AllAcceptorsHadNoProposal(cps, opn) {
-                forall rp | rp in ref_cps
-                    ensures !(ref_opn in rp.msg.votes)
-                {
-                    reveal_AbstractifyCVotesToVotes();
-                    var p :| p in cps && rp == AbstractifyCPacketToRslPacket(p);
-                    if ref_opn in rp.msg.votes {
-                        assert opn in p.msg.votes.v;
-                        assert false;
-                    }
-                }
-
-            }
-        }
-
-        forall opn | COperationNumberIsAbstractable(opn) 
-            ensures !AllAcceptorsHadNoProposal(cps, opn) ==> !LAllAcceptorsHadNoProposal(ref_cps, AbstractifyCOperationNumberToOperationNumber(opn));
-        {
-            var ref_opn := AbstractifyCOperationNumberToOperationNumber(opn);
-            if !AllAcceptorsHadNoProposal(cps, opn) {
-                assert !(forall p :: p in cps ==> !(opn in p.msg.votes.v));
-                var p :| p in cps && opn in p.msg.votes.v;
-                var ref_p := AbstractifyCPacketToRslPacket(p);
-
-                reveal_AbstractifyCVotesToVotes();
-
-                assert ref_p in ref_cps;
-            }
-        }
-    }
-
-//    calc ==> {
-//        SetOfMessage1b(cps);
-//            { reveal_AbstractifySetOfCPacketsToSetOfRslPackets(); }
-//        LSetOfMessage1b(AbstractifySetOfCPacketsToSetOfRslPackets(cps));
-//    }
-//    calc ==> {
-//        true;
-//            { reveal_AbstractifySetOfCPacketsToSetOfRslPackets(); }
-//        AbstractifySetOfCPacketsToSetOfRslPackets({}) == {};
-//    }
+//  calc ==> {
+//    SetOfMessage1b(cps);
+//      { reveal AbstractifySetOfCPacketsToSetOfRslPackets(); }
+//    LSetOfMessage1b(AbstractifySetOfCPacketsToSetOfRslPackets(cps));
+//  }
+//  calc ==> {
+//    true;
+//      { reveal AbstractifySetOfCPacketsToSetOfRslPackets(); }
+//    AbstractifySetOfCPacketsToSetOfRslPackets({}) == {};
+//  }
 }
 
 // Name this accessor for the proof below
 function PacketSrc(pkt:CPacket) : EndPoint
 {
-    pkt.src      
+  pkt.src      
 }
 
 lemma lemma_Received1bBound(proposer:ProposerState)
-    requires ProposerIsValid(proposer);
-    ensures  |proposer.received_1b_packets| < 0xFFFF_FFFF_FFFF_FFFF;
+  requires ProposerIsValid(proposer)
+  ensures  |proposer.received_1b_packets| < 0xFFFF_FFFF_FFFF_FFFF
 {
-    var srcs := set pkt | pkt in proposer.received_1b_packets :: PacketSrc(pkt);
+  var srcs := set pkt | pkt in proposer.received_1b_packets :: PacketSrc(pkt);
 
-    reveal_Received1bProperties();
-    lemma_MapSetCardinalityOver(proposer.received_1b_packets, srcs, PacketSrc);
-    assert |srcs| == |proposer.received_1b_packets|;
-    var replicas := UniqueSeqToSet(proposer.constants.all.config.replica_ids);
-    lemma_seqs_set_cardinality(proposer.constants.all.config.replica_ids, replicas);
-    SubsetCardinality(srcs, replicas);
+  reveal Received1bProperties();
+  lemma_MapSetCardinalityOver(proposer.received_1b_packets, srcs, PacketSrc);
+  assert |srcs| == |proposer.received_1b_packets|;
+  var replicas := UniqueSeqToSet(proposer.constants.all.config.replica_ids);
+  lemma_seqs_set_cardinality(proposer.constants.all.config.replica_ids, replicas);
+  SubsetCardinality(srcs, replicas);
 }
 
 } 
