ironfleet/src/Dafny/Distributed/Impl/RSL/Unsendable.i.dfy
@@ -2,21 +2,26 @@ include "../../Protocol/RSL/Replica.i.dfy"
 include "PacketParsing.i.dfy"
 
 module LiveRSL__Unsendable_i {
-    import opened LiveRSL__Replica_i
-    import opened LiveRSL__PacketParsing_i
+import opened Native__Io_s
+import opened Native__NativeTypes_s
+import opened LiveRSL__Replica_i
+import opened LiveRSL__PacketParsing_i
+import opened Common__GenericMarshalling_i
+import opened Environment_s
 
-    predicate IosReflectIgnoringUnsendable(ios:seq<LIoOp<EndPoint, seq<byte>>>)
-    {
-           |ios| == 1
-        && ios[0].LIoOpReceive?
-        && (   !Demarshallable(ios[0].r.msg, CMessage_grammar())
-            || !Marshallable(parse_Message(DemarshallFunc(ios[0].r.msg, CMessage_grammar()))))
-    }
+predicate IosReflectIgnoringUnsendable(ios:seq<LIoOp<EndPoint, seq<byte>>>)
+{
+  && |ios| == 1
+    && ios[0].LIoOpReceive?
+    && (|| !Demarshallable(ios[0].r.msg, CMessage_grammar())
+       || !Marshallable(parse_Message(DemarshallFunc(ios[0].r.msg, CMessage_grammar()))))
+}
     
-    predicate HostNextIgnoreUnsendable(s:LScheduler, s':LScheduler, ios:seq<LIoOp<EndPoint, seq<byte>>>)
-    {
-           s.nextActionIndex == 0
-        && s' == s.(nextActionIndex := 1)
-        && IosReflectIgnoringUnsendable(ios)
-    }
+predicate HostNextIgnoreUnsendable(s:LScheduler, s':LScheduler, ios:seq<LIoOp<EndPoint, seq<byte>>>)
+{
+  && s.nextActionIndex == 0
+  && s' == s.(nextActionIndex := 1)
+  && IosReflectIgnoringUnsendable(ios)
+}
+
 }
